rnm is pointwise differentially private

theories/diffpriv/examples/report_noisy_max.v
@@ -26,29 +26,298 @@ Section rnm.
     λ:"evalQ" "N" "d",
       let: "maxI" := ref #(-1) in
       let: "maxA" := ref #0 in
-      let: "cur" := ref #0 in
       let: "f" :=
         (rec: "rnm" "i" :=
            if: "i" = "N" then
              ! "maxI"
            else
              (let: "a" := Laplace #num #(2*den) ("evalQ" "i" "d") in
-              "cur" <- "a" ;;
-              (if: (* (! "maxI" = #(-1)) `or` *) (! "maxA" < "a") then
+              (if: ! "maxA" < "a" then
                  "maxA" <- "a" ;;
                  "maxI" <- "i"
                else #()) ;;
               "rnm" ("i" + #1)))
       in "f" #0.
 
-  Definition rnm_body (num den : Z) (evalQ : val) {DB} (dDB : Distance DB) (N : nat) (db : DB) (maxI maxA cur : loc) :=
+  Definition rnm_body (num den : Z) (evalQ : val) {DB} (dDB : Distance DB) (N : nat) (db : DB) (maxI maxA : loc) :=
     (rec: "rnm" "i" :=
        if: "i" = #N then ! #maxI
        else let: "a" := Laplace #num #(2*den) (evalQ "i" (inject db)) in
-            #cur <- "a" ;;
             (if: (* ! #maxI = #(-1) `or` *) ! #maxA < "a"
              then #maxA <- "a";; #maxI <- "i" else #());;
             "rnm" ("i" + #1))%V.
+
+  (* Definition rwp (e e' : expr) E (R : val → val → iProp Σ) : iProp Σ :=
+       (⤇ e' -∗ WP e @ E {{ v, ∃ v', R v v' }})%I.
+
+     (* Notation "'RWP' e ~ e' {{ Φ } } " := (rwp e e' top Φ) (only parsing).
+        Notation "'RWP' e ~ e' @ E {{ Φ } } " := (rwp e e' E Φ) (only parsing). *)
+     (* Notation "'RWP' e ~ e' @ E {{ v v' , Φ } } " := (rwp e e' E (λ v v', Φ)). *)
+
+     Notation "'RWP' e << e' {{ v , v' , Φ } } " := (rwp e e' top (λ v v', Φ))
+       (at level 20, e, e', Φ at level 200,
+      format "'[hv' 'RWP'  e  <<  e'  '/' {{  '[' v ,  v' ,  Φ  ']' } } ']'") : bi_scope.
+
+     Lemma pweq (e e' : expr) :
+       (⊢ RWP e << e' {{ v , v' ,  ⌜ v = v' ⌝ }})
+       →
+       (∀ x : val, ⤇ e' ⊢ WP e {{ v, ∃ v', ⤇ (of_val v') ∗ ⌜v = x -> v' = x⌝}})
+       →
+         (⤇ e' ⊢ WP e {{ v, ∃ v', ⤇ (of_val v') ∗ ⌜v = v'⌝ }}). *)
+
+  Lemma pweq (e e' : expr) K :
+    (∀ x : Z, ⤇ fill K e' -∗ WP e {{ v, ∃ v', ⤇ fill K (of_val v') ∗ ⌜v = #x -> v' = #x⌝}})
+    -∗
+    ({{{ ⤇ fill K e'}}} e {{{ (v : Z), RET #v; ⤇ fill K (of_val #v) }}}).
+  Admitted.
+
+
+  Lemma rnm_pw_diffpriv num den (evalQ : val) DB (dDB : Distance DB) (N : nat) K :
+    (0 < IZR num / IZR (2 * den)) →
+    (∀ i : Z, wp_sensitive (evalQ #i) 1 dDB dZ) →
+    ∀ db db', dDB db db' <= 1 →
+              ∀ j : nat,
+                {{{ ↯ (IZR num / IZR den) ∗
+                    ⤇ fill K (report_noisy_max num den evalQ #N (inject db')) }}}
+                  report_noisy_max num den evalQ #N (inject db)
+                  {{{ v, RET v ; ∃ v', ⤇ fill K v' ∗ ⌜ v = #j → v' = #j ⌝  }}}
+  .
+  Proof with (tp_pures ; wp_pures).
+    intros εpos qi_sens.
+    iIntros (db db' db_adj j Φ) "(ε & rnm) HΦ".
+    rewrite /report_noisy_max.
+    simpl. tp_pures. wp_pures.
+    (* initialize *)
+    tp_alloc as maxI2 "maxI2". tp_pures. tp_alloc as maxA2 "maxA2". do 5 tp_pure.
+    wp_pures. wp_alloc maxI1 as "maxI1". wp_alloc maxA1 as "maxA1". do 5 wp_pure.
+    rewrite -/(rnm_body num den evalQ dDB N db maxI1 maxA1).
+    rewrite -/(rnm_body num den evalQ dDB N db' maxI2 maxA2).
+    (* generalize loop variable, set up invariants *)
+    cut
+      (∀ (i imax1 imax2 : Z) (amax1 amax2 : Z),
+          {{{ maxI1 ↦ #imax1 ∗ maxI2 ↦ₛ #imax2 ∗ maxA1 ↦ #amax1 ∗ maxA2 ↦ₛ #amax2
+              ∗ ↯ (if (bool_decide (i <= j))%Z then (IZR num / IZR den) else 0)
+              ∗ ⤇ fill K (rnm_body num den evalQ dDB N db' maxI2 maxA2 #i)
+              ∗ ⌜ 0 <= i <= N ⌝%Z
+              ∗ ⌜ i < j
+                  → ((dZ amax1 amax2 <= 1)%R
+                     ∧ imax1 < i ∧ imax2 < i
+                     ∧ ((¬ (i <= N ∧ i < j)) → i = j)
+                ) ⌝%Z
+              ∗ ⌜ i = j
+                  → ( (dZ amax1 amax2 <= 1)%R
+                      ∧ (imax1 = j → (imax2 = j ∧ amax1 + 1 = amax2))
+                      ∧ (¬ (i <= N ∧ i = j) → i = j+1) )%Z ⌝
+              ∗ ⌜ (j < i)%Z
+                  → ( imax1 = j → (imax2 = j ∧ amax1 + 1 = amax2) )%Z ⌝
+          }}}
+            rnm_body num den evalQ dDB N db maxI1 maxA1 #i
+            {{{ (v : Z), RET #v;
+                ∃ (v' : Z), ⤇ fill K #v' ∗ ⌜ v = j -> v' = j ⌝
+            }}}
+      ).
+    (* the general statement implies the original goal *)
+    1: { intros h.
+         iMod ec_zero as "ε0".
+         iApply (h with "[-HΦ]").
+         - (* We have all the reference resources for the IH. *)
+           iFrame.
+           iSplitL.
+           (* We have the error credits too *)
+           + case_bool_decide ; iFrame.
+           (* and the arithmetic works out fine *)
+           + iPureIntro. split ; [|split ; [|split]]. 1: lia.
+             * clear. intros. repeat split.
+               -- rewrite distance_0 ; lra.
+               -- intros []. lia.
+             * clear. intros. repeat split. all: try lia.
+               -- rewrite distance_0 ; lra.
+             * clear. intros. lia.
+         - (* The post-condition of the IH implies the original post. *)
+           iNext ; iIntros (v) "(%v' & v' & %h')".
+           iApply "HΦ". iExists _. iFrame.
+           iPureIntro. intro h''. do 3 f_equal. apply h'. inversion h''. done.
+    }
+    clear Φ.
+
+    (* the actual induction begins *)
+    iLöb as "IH".
+    iIntros (i imax1 imax2 amax1 amax2 Φ) "(maxI1 & maxI2 & maxA1 & maxA2 & ε & rnm' & %iN & %below_j & %at_j & %above_j) HΦ".
+    rewrite {4}/rnm_body. wp_pures.
+    rewrite {3}/rnm_body. tp_pures ; [cbv ; auto|].
+    case_bool_decide (#i = #N) as iN'.
+
+    (* base case *)
+    - tp_pures. wp_pures. tp_load ; wp_load. iApply "HΦ". iExists imax2. iFrame "rnm'". iPureIntro.
+      intros ij1. inversion iN'.
+      subst. clear -below_j at_j above_j.
+      lia.
+
+    (* rnm body *)
+    - assert (i ≠ N). { intro h. apply iN'. subst. done. }
+      assert (i < N)%Z by lia.
+      tp_pures ; wp_pures.
+      rewrite -/(rnm_body _ _ _ _ _ _ _ maxA1).
+      rewrite -/(rnm_body _ _ _ _ _ _ _ maxA2).
+
+      (* sensitivity of evalQ *)
+      tp_bind (evalQ _ _). wp_bind (evalQ _ _).
+      rewrite /wp_sensitive in qi_sens.
+      iApply (qi_sens i _ _ db db' _ with "rnm'").
+      Unshelve. 2: lra.
+      iIntros "!> % (%e1 & %e2 & -> & rnm' & %e1e2_adj)" => /=.
+      assert (-1 <= e1 - e2 <= 1)%Z as [].
+      {
+        rewrite Rmult_1_l in e1e2_adj.
+        assert (dZ e1 e2 <= 1) as h by (etrans ; eauto).
+        revert h.
+        rewrite /dZ/distance Rabs_Zabs.
+        apply Zabs_ind ; intros ? h; split.
+        all: pose proof (le_IZR _ _ h) ; lia.
+      }
+
+      (* case on the whether i is below, at, or above the result j. *)
+      destruct (Z.lt_trichotomy i j) as [ij | [e|ij]].
+      2:{                       (* i = j *)
+        tp_bind (Laplace _ _ _).
+        wp_bind (Laplace _ _ _).
+        iApply (wp_couple_laplace e1 e2 1%Z 2%Z with "[$rnm' ε]") => //.
+        1: apply Zabs_ind ; lia.
+        { case_bool_decide. 2: lia.
+          iApply ec_eq. 2: iFrame.
+          rewrite /Rdiv. rewrite mult_IZR. field. clear -εpos.
+          intro d0.
+          rewrite mult_IZR in εpos.
+          rewrite Rdiv_mult_distr in εpos.
+          rewrite d0 in εpos.
+          rewrite Rdiv_0_r in εpos.
+          lra.
+        }
+        iNext ; iIntros (a) "rnm'" => /=.
+        wp_pures. tp_pures.
+        tp_load ; wp_load ; tp_pures ; wp_pures.
+        specialize (at_j e). destruct at_j as (amax_adj & jmax1 & inext).
+        case_bool_decide (amax1 < a)%Z as case_l ; tp_pures ; wp_pures.
+        all: case_bool_decide as case_r ; tp_pures ; wp_pures.
+        * do 2 (tp_store ; tp_pures ; wp_store ; wp_pures).
+          iMod ec_zero as "ε0".
+          iApply ("IH" with "[-HΦ]") ; iFrame.
+          rewrite e. case_bool_decide ; try lia. iFrame.
+          iPureIntro. intuition lia.
+        * exfalso. clear -case_l case_r amax_adj.
+          assert (a+1 <= amax2)%Z by lia.
+          revert amax_adj.
+          rewrite /dZ/distance Rabs_Zabs. apply Zabs_ind ; intros.
+          -- lia.
+          -- pose proof (le_IZR _ _ amax_adj). lia.
+        * iMod ec_zero as "ε0".
+          tp_store ; tp_pures ; tp_store ; tp_pures.
+          iSpecialize ("IH" $! (i+1)%Z imax1 i amax1 (a+1)%Z).
+          iSpecialize ("IH" with "[ε0 $rnm' $maxA1 $maxA2 $maxI1 $maxI2]").
+          2: iApply ("IH" with "[HΦ]") ; iFrame.
+          iSplitL. 1: case_bool_decide ; try lia ; iFrame "ε0".
+          iPureIntro ; intuition lia.
+        * iMod ec_zero as "ε0".
+          iApply ("IH" with "[-HΦ]") ; iFrame.
+          rewrite e. case_bool_decide ; try lia. iFrame.
+          iFrame. iPureIntro. intuition lia.
+      }
+
+      (* i < j *)
+      {
+        destruct (below_j ij) as (amax_adj & imax1i & imax2i & inext).
+        tp_bind (Laplace _ _ _).
+        wp_bind (Laplace _ _ _).
+        iMod ec_zero as "ε0".
+        iApply (wp_couple_laplace e1 e2 (e2 - e1)%Z 0%Z with "[$rnm' ε0]") => //.
+        1: eapply Zabs_ind ; intuition lia.
+        1: rewrite Rmult_0_l => //.
+        iNext ; iIntros (a) "rnm'" => /=.
+        wp_pures. tp_pures.
+        tp_load ; wp_load ; tp_pures ; wp_pures.
+        case_bool_decide (amax1 < a)%Z as case_l.
+        all: case_bool_decide (amax2 < a + (e2 - e1))%Z as case_r.
+        all: tp_pures ; wp_pures.
+        - do 2 (tp_store ; tp_pures ; wp_store ; wp_pures).
+          iApply ("IH" with "[-HΦ]") ; iFrame.
+          iSplitL. 1: repeat case_bool_decide ; try lia ; iFrame.
+          iPureIntro.
+          intuition try lia.
+          all: rewrite /dZ/distance Rabs_Zabs ; apply Zabs_ind ; intros ; apply IZR_le ; intuition try lia.
+        - wp_store ; wp_pures ; wp_store ; wp_pures.
+          iApply ("IH" $! (i+1)%Z with "[-HΦ]") ; iFrame.
+          iSplitL. 1: repeat case_bool_decide ; try lia ; iFrame.
+          assert (a+(e2-e1) <= amax2)%Z by lia.
+          rewrite /dZ/distance Rabs_Zabs.
+          all: iPureIntro ; repeat split ; try by intuition lia.
+          + apply IZR_le.
+            revert amax_adj. rewrite /dZ/distance Rabs_Zabs.
+            apply Zabs_ind ; intros ; pose proof (le_IZR _ _ amax_adj).
+            all: apply Zabs_ind ; intros ; lia.
+          + apply IZR_le.
+            revert amax_adj. rewrite /dZ/distance Rabs_Zabs.
+            apply Zabs_ind ; intros ; pose proof (le_IZR _ _ amax_adj).
+            all: apply Zabs_ind ; intros ; lia.
+        - tp_store ; tp_pures ; tp_store ; tp_pures.
+          iApply ("IH" $! (i+1)%Z with "[-HΦ]") ; iFrame.
+          iSplitL. 1: repeat case_bool_decide ; try lia ; iFrame.
+          assert (a <= amax1)%Z by lia.
+          rewrite /dZ/distance Rabs_Zabs.
+          all: iPureIntro ; repeat split ; try by intuition lia.
+          + apply IZR_le.
+            revert amax_adj.
+            rewrite /dZ/distance Rabs_Zabs.
+            apply Zabs_ind ; intros.
+            all: pose proof (le_IZR _ _ amax_adj).
+            all: apply Zabs_ind ; intros ; lia.
+          + apply IZR_le.
+            revert amax_adj.
+            rewrite /dZ/distance Rabs_Zabs.
+            apply Zabs_ind ; intros.
+            all: pose proof (le_IZR _ _ amax_adj).
+            all: apply Zabs_ind ; intros ; lia.
+        - iApply ("IH" $! (i+1)%Z with "[-HΦ]") ; iFrame.
+          iSplitL. 1: repeat case_bool_decide ; try lia ; iFrame.
+          all: iPureIntro ; repeat split ; try by intuition lia.
+      }
+      (* j < i *)
+      {
+        specialize (above_j ij).
+        tp_bind (Laplace _ _ _).
+        wp_bind (Laplace _ _ _).
+        iMod ec_zero as "ε0".
+        iApply (wp_couple_laplace e1 e2 (e2 - e1)%Z 0%Z with "[$rnm' ε0]") => //.
+        1: eapply Zabs_ind ; intuition lia.
+        1: rewrite Rmult_0_l => //.
+        iNext ; iIntros (a) "rnm'" => /=.
+        wp_pures. tp_pures.
+
+        tp_load ; wp_load ; tp_pures ; wp_pures.
+
+        case_bool_decide (amax1 < a)%Z as case_l.
+        all: case_bool_decide (amax2 < a + (e2 - e1))%Z as case_r.
+        all: tp_pures ; wp_pures.
+        - do 2 (tp_store ; tp_pures ; wp_store ; wp_pures).
+          iApply ("IH" with "[-HΦ]") ; iFrame.
+          iSplitL. 1: repeat case_bool_decide ; try lia ; iFrame.
+          iPureIntro.
+          intuition try lia.
+        - wp_store ; wp_pures ; wp_store ; wp_pures.
+          iApply ("IH" $! (i+1)%Z with "[-HΦ]") ; iFrame.
+          iSplitL. 1: repeat case_bool_decide ; try lia ; iFrame.
+          all: iPureIntro ; repeat split ; try by intuition lia.
+        - tp_store ; tp_pures ; tp_store ; tp_pures.
+          iApply ("IH" $! (i+1)%Z with "[-HΦ]") ; iFrame.
+          iSplitL. 1: repeat case_bool_decide ; try lia ; iFrame.
+          all: iPureIntro ; repeat split ; try by intuition lia.
+        - iApply ("IH" $! (i+1)%Z with "[-HΦ]") ; iFrame.
+          iSplitL. 1: repeat case_bool_decide ; try lia ; iFrame.
+          all: iPureIntro ; repeat split ; try by intuition lia.
+      }
+  Qed.
+
+
+  (* sketchy concrete example below *)
 
   Definition DB := (Z * Z * Z)%type.
   Definition dDB : Distance DB.
@@ -90,702 +359,83 @@ Section rnm.
                 else if: "i" = #1 then count_over_80 "db"
                      else #0.
 
-  (* Definition rwp (e e' : expr) E (R : val → val → iProp Σ) : iProp Σ :=
-       (⤇ e' -∗ WP e @ E {{ v, ∃ v', R v v' }})%I.
-
-     (* Notation "'RWP' e ~ e' {{ Φ } } " := (rwp e e' top Φ) (only parsing).
-        Notation "'RWP' e ~ e' @ E {{ Φ } } " := (rwp e e' E Φ) (only parsing). *)
-     (* Notation "'RWP' e ~ e' @ E {{ v v' , Φ } } " := (rwp e e' E (λ v v', Φ)). *)
-
-     Notation "'RWP' e << e' {{ v , v' , Φ } } " := (rwp e e' top (λ v v', Φ))
-       (at level 20, e, e', Φ at level 200,
-      format "'[hv' 'RWP'  e  <<  e'  '/' {{  '[' v ,  v' ,  Φ  ']' } } ']'") : bi_scope.
-
-     Lemma pweq (e e' : expr) :
-       (⊢ RWP e << e' {{ v , v' ,  ⌜ v = v' ⌝ }})
-       →
-       (∀ x : val, ⤇ e' ⊢ WP e {{ v, ∃ v', ⤇ (of_val v') ∗ ⌜v = x -> v' = x⌝}})
-       →
-         (⤇ e' ⊢ WP e {{ v, ∃ v', ⤇ (of_val v') ∗ ⌜v = v'⌝ }}). *)
-
-  Lemma pweq_weak (e e' : expr) K :
-    (⊢ (⤇ e' -∗ WP e {{ v, ∃ v', ⤇ (of_val v')}}))
-    →
-      (⤇ fill K e' -∗ WP e {{ v, (∃ z : Z, ⌜v = #z⌝)
-                                 ∗ ∃ v', ⤇ fill K (of_val v') ∗ ⌜∀ x : Z, v = #x -> v' = #x⌝}})
-      -∗
-    (⤇ fill K e' -∗ WP e {{ v, ∃ z : Z, ⌜v = #z⌝ ∗ ⤇ fill K (of_val v) }}).
-  Proof.
-    iIntros (?) "h Ke'".
-    iSpecialize ("h" with "Ke'").
-    iApply (wp_mono with "h").
-    iIntros (v) "((%z & %eq_v_z) & %v' & Kv' & %alleq)".
-    iExists z. rewrite (alleq _ eq_v_z). rewrite eq_v_z. iFrame. done.
-  Qed.
-
-
-  (* Lemma pweq (e e' : expr) K :
-       (* (⊢ (⤇ e' -∗ WP e {{ v, ∃ v', ⤇ (of_val v')}}))
-          → *)
-       ∀ x : Z,
-       ( ⤇ fill K e' -∗ WP e {{ v, ∃ v', ⤇ fill K (of_val v') ∗ ⌜v = #x -> v' = #x⌝}})
-       -∗
-         (⤇ fill K e' -∗ WP e {{ v, ∃ z : Z, ⌜v = #z⌝ ∗ ⤇ fill K (of_val v) }}).
-     (* Admitted. *)
+  (* concrete example run *)
+  (* Lemma rnm_diffpriv_3 num den :
+       (0 < IZR num / IZR den) →
+       ∀ (K : list (ectxi_language.ectx_item prob_ectxi_lang)),
+         {{{ ⤇ fill K (report_noisy_max num den evalQ #2 (inject db')) ∗
+             ↯ (IZR num / IZR den)
+               (* ↯ 0 *)
+         }}}
+           (report_noisy_max num den evalQ #2 (inject db))
+           {{{ (v : val), RET v; ⤇ fill K v }}}.
      Proof.
-       intros x. iIntros "alleq e'".
-       (* iDestruct (safe with "[$e']") as "H". *)
-       iDestruct ("alleq" with "[$e']") as "H".
-       iApply (wp_mono with "H").
-       iIntros (v) "(%v' & v' & %h)".
-       iExists _.
-       rewrite h.
-       iSplitR ; [iPureIntro|]. *)
-  Lemma pweq (e e' : expr) K :
-    (∀ x : Z, ⤇ fill K e' -∗ WP e {{ v, ∃ v', ⤇ fill K (of_val v') ∗ ⌜v = #x -> v' = #x⌝}})
-    -∗
-    ({{{ ⤇ fill K e'}}} e {{{ (v : Z), RET #v; ⤇ fill K (of_val #v) }}}).
-  Admitted.
+       iIntros (???) "[rnm' ε] hφ".
+       rewrite /report_noisy_max.
+       simpl.
+       tp_pures.
+       tp_alloc as maxI2 "maxI2". tp_pures. tp_alloc as maxA2 "maxA2". do 5 tp_pure.
+       wp_pures. wp_alloc maxI1 as "maxI1". wp_alloc maxA1 as "maxA1". do 5 wp_pure.
+       wp_rec. wp_pures.
+       tp_pures. 1: cbv ; auto.
+       rewrite {2 4}/evalQ. tp_pures. 1: cbv ; auto. wp_pures.
+       rewrite /count_under_40/setsum/setmap/under_40/age. wp_pures. tp_pures.
 
-
-  Goal forall (N : nat), {{{ ⌜True⌝ }}} (rec: "f" "i" := if: "i" = #N then #42 else "f" ("i" + #1)) #0 {{{v, RET #v; ⌜v = 42%Z⌝}}}.
-    intros. iIntros "_ h". wp_pure.
-    cut (∀ i : Z, ⌜0 <= i <= N ⌝%Z ⊢ WP (rec: "f" "i" := if: "i" = #N then #42 else "f" ("i" + #1))%V #i {{ v, ⌜ v = #42 ⌝ }}).
-    { intros h. iPoseProof (h 0%Z) as "hh".
-      iApply wp_strong_mono'. 1: auto. 1: iApply "hh". 1: iPureIntro ; lia.
-      iIntros (????) "[? [? [? ->]]]" ; iFrame. iModIntro. iApply "h".
-      done.
-    }
-    iLöb as "IH". iIntros (i) "%iN".
-    wp_pures. case_bool_decide.
-    - wp_pures. done.
-    - wp_pure. wp_pure. iApply "IH".
-      assert (i ≠ N). { intro. apply H. subst. done. }
-      iPureIntro.
-      lia.
-  Qed.
-
-  Lemma rnm_pw_diffpriv num den (evalQ : val) DB (dDB : Distance DB) (N : nat) K :
-    (0 < IZR num / IZR (2 * den)) →
-    (∀ i : Z, wp_sensitive (evalQ #i) 1 dDB dZ) →
-    ∀ db db', dDB db db' <= 1 →
-              ∀ j : nat,
-                {{{ ↯ (IZR num / IZR den) ∗
-                    ⤇ fill K (report_noisy_max num den evalQ #N (inject db')) }}}
-                  report_noisy_max num den evalQ #N (inject db)
-                  {{{ v, RET v ; ∃ v', ⤇ fill K v' ∗ ⌜ v = #j → v' = #j ⌝  }}}
-  .
-  Proof with (tp_pures ; wp_pures).
-    intros εpos qi_sens.
-    iIntros (db db' db_adj x Φ) "(ε & rnm) HΦ".
-    rewrite /report_noisy_max.
-    simpl.
-    tp_pures.
-    wp_pures.
-    tp_alloc as maxI2 "maxI2". tp_pures. tp_alloc as maxA2 "maxA2". tp_pures. tp_alloc as cur2 "cur2".  do 5 tp_pure.
-    wp_pures. wp_alloc maxI1 as "maxI1". wp_alloc maxA1 as "maxA1". wp_alloc cur1 as "cur1".  do 5 wp_pure.
-    rewrite -/(rnm_body num den evalQ dDB N db maxI1 maxA1 cur1).
-    rewrite -/(rnm_body num den evalQ dDB N db' maxI2 maxA2 cur2).
-    rename x into j.
-    cut
-      (∀ (i imax1 imax2 : Z) (amax1 amax2 vcur1 vcur2 : Z),
-          {{{ maxI1 ↦ #imax1 ∗ maxI2 ↦ₛ #imax2 ∗ maxA1 ↦ #amax1 ∗ maxA2 ↦ₛ #amax2
-              ∗ cur1 ↦ #vcur1 ∗ cur2 ↦ₛ #vcur2
-              ∗ ↯ (if (bool_decide (i <= j))%Z then (IZR num / IZR den) else 0)
-              ∗ ⤇ fill K (rnm_body num den evalQ dDB N db' maxI2 maxA2 cur2 #i)
-              ∗ ⌜ 0 <= i <= N ⌝%Z
-              ∗ ⌜ i < j
-                  → ((dZ amax1 amax2 <= 1)%R
-                     ∧ imax1 < i ∧ imax2 < i
-                     ∧ ((¬ (i <= N ∧ i < j)) → i = j)
-                ) ⌝%Z
-              ∗ ⌜ i = j
-                  → ( (dZ amax1 amax2 <= 1)%R
-                      ∧ (imax1 = j → (imax2 = j ∧ amax1 + 1 = amax2))
-                      ∧ (¬ (i <= N ∧ i = j) → i = j+1) )%Z ⌝
-              ∗ ⌜ (j < i)%Z
-                  → ( imax1 = j → (imax2 = j ∧ amax1 + 1 = amax2) )%Z ⌝
-          }}}
-            rnm_body num den evalQ dDB N db maxI1 maxA1 cur1 #i
-            {{{ (v : Z), RET #v;
-                ∃ (v' : Z), ⤇ fill K #v' ∗ ⌜ v = j -> v' = j ⌝
-            }}}
-      ).
-    1: { intros h.
-         iMod ec_zero as "ε0".
-         iApply (h with "[-HΦ]").
-         - (* We have all the reference resources for the IH. *)
-           iFrame.
-           iSplitL.
-           (* We have the error credits too *)
-           + case_bool_decide ; iFrame.
-           (* and the arithmetic works out fine *)
-           + iPureIntro. split ; [|split ; [|split]]. 1: lia.
-             * clear. intros. repeat split.
-               -- rewrite distance_0 ; lra.
-               -- intros []. lia.
-             * clear. intros. repeat split. all: try lia.
-               -- rewrite distance_0 ; lra.
-             * clear. intros. lia.
-         - (* The post-condition of the IH implies the original post. *)
-           iNext ; iIntros (v) "(%v' & v' & %h')".
-           iApply "HΦ". iExists _. iFrame.
-           iPureIntro. intro h''. do 3 f_equal. apply h'. inversion h''. done.
-    }
-    clear Φ.
-    iLöb as "IH".
-    iIntros (i imax1 imax2 amax1 amax2 vcur1 vcur2 Φ) "(maxI1 & maxI2 & maxA1 & maxA2 & cur1 & cur2 & ε & rnm' & %iN & %below_j & %at_j & %above_j) HΦ".
-    rewrite {4}/rnm_body. wp_pures.
-    rewrite {3}/rnm_body. tp_pures ; [cbv ; auto|].
-    case_bool_decide (#i = #N) as iN'.
-    - tp_pures. wp_pures. tp_load ; wp_load. iApply "HΦ". iExists imax2. iFrame "rnm'". iPureIntro.
-      intros ij1. inversion iN'.
-      try lia.
-    -
-      assert (i ≠ N). { intro h. apply iN'. subst. done. }
-      assert (i < N)%Z by lia.
-      tp_pures ; wp_pures.
-      rewrite -/(rnm_body _ _ _ _ _ _ _ maxA1 _).
-      rewrite -/(rnm_body _ _ _ _ _ _ _ maxA2 _).
-      tp_bind (evalQ _ _).
-      wp_bind (evalQ _ _).
-
-      rewrite /wp_sensitive in qi_sens.
-      opose proof (qi_sens i _ _ db db') as ev ; [lra|].
-      iApply (ev with "rnm'").
-      iIntros "!> % (%e1 & %e2 & -> & rnm' & %e1e2_adj)" => /=.
-
-      assert (-1 <= e1 - e2 <= 1)%Z as [].
-      {
-        rewrite Rmult_1_l in e1e2_adj.
-        assert (dZ e1 e2 <= 1) as h by (etrans ; eauto).
-        revert h.
-        rewrite /dZ/distance Rabs_Zabs.
-        apply Zabs_ind ; intros ? h; split.
-        all: pose proof (le_IZR _ _ h) ; lia.
-      }
-
-      destruct (make_decision (i = j)) as [e|n].
-      + tp_bind (Laplace _ _ _).
-        wp_bind (Laplace _ _ _).
-        iApply (wp_couple_laplace e1 e2 1%Z 2%Z with "[$rnm' ε]") => //.
-        { apply Zabs_ind ; lia. }
-        { case_bool_decide. 2: lia.
-          iApply ec_eq. 2: iFrame.
-          rewrite /Rdiv. rewrite mult_IZR. rewrite Rinv_mult.
-          field. clear -εpos.
-          intro d0.
-          rewrite mult_IZR in εpos.
-          rewrite Rdiv_mult_distr in εpos.
-          rewrite d0 in εpos.
-          rewrite Rdiv_0_r in εpos.
-          lra.
-        }
-        iNext ; iIntros (a) "rnm'" => /=.
-        wp_pures. tp_pures.
-        (* rewrite !Zplus_0_r. *)
-        tp_store ; tp_pures ; wp_store.
-        tp_load ; wp_load ; tp_pures ; wp_pures.
-        specialize (at_j e). destruct at_j as (amax_adj & jmax1 & inext).
-        case_bool_decide (amax1 < a)%Z as case_l ; tp_pures ; wp_pures.
-        all: case_bool_decide as case_r ; tp_pures ; wp_pures.
-        * do 2 (tp_store ; tp_pures ; wp_store ; wp_pures).
-          iMod ec_zero as "ε0".
-          iApply ("IH" with "[-HΦ]") ; iFrame.
-          rewrite e. case_bool_decide ; try lia. iFrame.
-          iPureIntro.
-
-          split ; [| split ; [|split] ]. 1,2,3: lia.
-          intros. split => //.
-        *
-          exfalso. clear -case_l case_r amax_adj.
-          assert (a+1 <= amax2)%Z by lia.
-          revert amax_adj.
-          rewrite /dZ/distance Rabs_Zabs. apply Zabs_ind ; intros.
-          -- lia.
-          -- pose proof (le_IZR _ _ amax_adj). lia.
-        *
-          iMod ec_zero as "ε0".
-          tp_store ; tp_pures ; tp_store ; tp_pures.
-          iSpecialize ("IH" $! (i+1)%Z imax1 i amax1 (a+1)%Z a (a+1)%Z).
-          iSpecialize ("IH" with "[ε0 $rnm' $maxA1 $maxA2 $maxI1 $maxI2 $cur1 $cur2]").
-          2: iApply ("IH" with "[HΦ]") ; iFrame.
-          iSplitL. 1: case_bool_decide ; try lia ; iFrame "ε0".
-          iPureIntro ; split ; [|split; [|split]].
-          1,2,3: by intuition lia.
-          intros.
-          split => //. lia.
-
-        * iMod ec_zero as "ε0".
-          iApply ("IH" with "[-HΦ]") ; iFrame.
-          rewrite e. case_bool_decide ; try lia. iFrame.
-          iFrame. iPureIntro. intuition lia.
-
-      + destruct (Z.lt_trichotomy i j) as [ij | [ij|ij]]. 2: by exfalso.
-
-        *
-          destruct (below_j ij) as (amax_adj & imax1i & imax2i & inext).
-          tp_bind (Laplace _ _ _).
-          wp_bind (Laplace _ _ _).
-          iMod ec_zero as "ε0".
-          iApply (wp_couple_laplace e1 e2 (e2 - e1)%Z 0%Z with "[$rnm' ε0]") => //.
-          {
-            eapply Zabs_ind ; intuition lia.
-          }
-          1: rewrite Rmult_0_l => //.
-          iNext ; iIntros (a) "rnm'" => /=.
-          wp_pures. tp_pures. tp_store ; tp_pures ; wp_store.
-          tp_load ; wp_load ; tp_pures ; wp_pures.
-
-          case_bool_decide (amax1 < a)%Z as case_l.
-          all: case_bool_decide (amax2 < a + (e2 - e1))%Z as case_r.
-          all: tp_pures ; wp_pures.
-
-          -- do 2 (tp_store ; tp_pures ; wp_store ; wp_pures).
-             iApply ("IH" with "[-HΦ]") ; iFrame.
-             iSplitL. 1: repeat case_bool_decide ; try lia ; iFrame.
-             iPureIntro.
-             intuition try lia.
-             all: rewrite /dZ/distance Rabs_Zabs ; apply Zabs_ind ; intros ; apply IZR_le ; intuition try lia.
-          -- wp_store ; wp_pures ; wp_store ; wp_pures.
-             iApply ("IH" $! (i+1)%Z with "[-HΦ]") ; iFrame.
-             iSplitL. 1: repeat case_bool_decide ; try lia ; iFrame.
-             assert (a+(e2-e1) <= amax2)%Z by lia.
-             rewrite /dZ/distance Rabs_Zabs.
-             all: iPureIntro ; repeat split ; try by intuition lia.
-             ++ apply IZR_le.
-               revert amax_adj. rewrite /dZ/distance Rabs_Zabs.
-               apply Zabs_ind ; intros ; pose proof (le_IZR _ _ amax_adj).
-               all: apply Zabs_ind ; intros ; lia.
-             ++ apply IZR_le.
-               revert amax_adj. rewrite /dZ/distance Rabs_Zabs.
-               apply Zabs_ind ; intros ; pose proof (le_IZR _ _ amax_adj).
-               all: apply Zabs_ind ; intros ; lia.
-          -- tp_store ; tp_pures ; tp_store ; tp_pures.
-             iApply ("IH" $! (i+1)%Z with "[-HΦ]") ; iFrame.
-             iSplitL. 1: repeat case_bool_decide ; try lia ; iFrame.
-             assert (a <= amax1)%Z by lia.
-             rewrite /dZ/distance Rabs_Zabs.
-             all: iPureIntro ; repeat split ; try by intuition lia.
-             ++ apply IZR_le.
-                revert amax_adj.
-                rewrite /dZ/distance Rabs_Zabs.
-                apply Zabs_ind ; intros.
-                all: pose proof (le_IZR _ _ amax_adj).
-                all: apply Zabs_ind ; intros ; lia.
-             ++ apply IZR_le.
-                revert amax_adj.
-                rewrite /dZ/distance Rabs_Zabs.
-                apply Zabs_ind ; intros.
-                all: pose proof (le_IZR _ _ amax_adj).
-                all: apply Zabs_ind ; intros ; lia.
-          -- iApply ("IH" $! (i+1)%Z with "[-HΦ]") ; iFrame.
-            iSplitL. 1: repeat case_bool_decide ; try lia ; iFrame.
-            all: iPureIntro ; repeat split ; try by intuition lia.
-
-        *
-          specialize (above_j ij).
-          tp_bind (Laplace _ _ _).
-          wp_bind (Laplace _ _ _).
-          iMod ec_zero as "ε0".
-          iApply (wp_couple_laplace e1 e2 (e2 - e1)%Z 0%Z with "[$rnm' ε0]") => //.
-          {
-            eapply Zabs_ind ; intuition lia.
-          }
-          1: rewrite Rmult_0_l => //.
-          iNext ; iIntros (a) "rnm'" => /=.
-          wp_pures. tp_pures. tp_store ; tp_pures ; wp_store.
-
-          tp_load ; wp_load ; tp_pures ; wp_pures.
-
-          case_bool_decide (amax1 < a)%Z as case_l.
-          all: case_bool_decide (amax2 < a + (e2 - e1))%Z as case_r.
-          all: tp_pures ; wp_pures.
-
-          -- do 2 (tp_store ; tp_pures ; wp_store ; wp_pures).
-             iApply ("IH" with "[-HΦ]") ; iFrame.
-             iSplitL. 1: repeat case_bool_decide ; try lia ; iFrame.
-             iPureIntro.
-             intuition try lia.
-          -- wp_store ; wp_pures ; wp_store ; wp_pures.
-             iApply ("IH" $! (i+1)%Z with "[-HΦ]") ; iFrame.
-             iSplitL. 1: repeat case_bool_decide ; try lia ; iFrame.
-             all: iPureIntro ; repeat split ; try by intuition lia.
-
-          -- tp_store ; tp_pures ; tp_store ; tp_pures.
-
-             iApply ("IH" $! (i+1)%Z with "[-HΦ]") ; iFrame.
-             iSplitL. 1: repeat case_bool_decide ; try lia ; iFrame.
-             all: iPureIntro ; repeat split ; try by intuition lia.
-          --
-            iApply ("IH" $! (i+1)%Z with "[-HΦ]") ; iFrame.
-            iSplitL. 1: repeat case_bool_decide ; try lia ; iFrame.
-            all: iPureIntro ; repeat split ; try by intuition lia.
-Qed.
-
-
-
-
-
-
-
-
-
-
-
-
-
-
-
-
-
-
-
-
-
-
-
-
-
-          Lemma rnm_diffpriv num den (evalQ : val) DB (dDB : Distance DB) (N : nat) :
-            (0 < IZR num / IZR den) →
-            (∀ i : Z, wp_sensitive (evalQ #i) 1 dDB dZ) →
-            wp_diffpriv (report_noisy_max num den evalQ #N) (IZR num / IZR den) dDB.
-          Proof with (tp_pures ; wp_pures).
-            intros εpos qi_sens.
-            iIntros (? c db db' db_adj Φ) "(rnm & ε) HΦ".
-            rewrite /report_noisy_max.
-            tp_pures.
-            tp_alloc as maxI2 "maxI2". tp_pures. tp_alloc as maxA2 "maxA2". tp_pures. tp_alloc as cur2 "cur2".  do 5 tp_pure.
-            wp_pures. wp_alloc maxI1 as "maxI1". wp_alloc maxA1 as "maxA1". wp_alloc cur1 as "cur1".  do 5 wp_pure.
-            rewrite -/(rnm_body num den evalQ dDB N db maxI1 maxA1 cur1).
-            rewrite -/(rnm_body num den evalQ dDB N db' maxI2 maxA2 cur2).
-            iApply (pweq with "[-HΦ rnm] [$rnm] [HΦ]"). 2: iNext ; iIntros ; iApply "HΦ" ; done.
-            clear Φ.
-            iIntros (x) "rnm'".
-
-            cut
-              (∀ (j i imax1 imax2 : Z) (amax1 amax2 vcur1 vcur2 : Z),
-                  {{{ maxI1 ↦ #imax1 ∗ maxI2 ↦ₛ #imax2 ∗ maxA1 ↦ #amax1 ∗ maxA2 ↦ₛ #amax2
-                      ∗ cur1 ↦ #vcur1 ∗ cur2 ↦ₛ #vcur2
-                      ∗ ↯ (if (bool_decide (i <= j))%Z then c * (IZR num / IZR den) else 0)
-                      ∗ ⤇ fill K (rnm_body num den evalQ dDB N db' maxI2 maxA2 cur2 #i)
-                      ∗ ⌜(amax1 < vcur1 → imax1 = i)%Z⌝
-                      ∗ ⌜(amax2 < vcur2 → imax1 = i)%Z⌝
-                      ∗ ⌜ imax1 = imax2 ⌝
-                      (* ∗ ⌜((i = N → imax1 = j → imax2 = j))%Z⌝ *)
-                      ∗ ⌜True%Z⌝
-                  }}}
-                    rnm_body num den evalQ dDB N db maxI1 maxA1 cur1 #i
-                    {{{ (v : Z), RET #v;
-                        ∃ (v' : Z), ⤇ fill K #v' ∗ ⌜ v = j -> v' = j ⌝
-                    }}}
-
-              ).
-
-            1: { intros h.
-                 iMod ec_zero as "ε0".
-                 iApply (h x with "[-]").
-                 - (* We have all the reference resources for the IH. *)
-                   iFrame.
-                   iSplitL.
-                   (* We have the error credits too *)
-                   + case_bool_decide ; iFrame.
-                   (* and the arithmetic works out fine *)
-                   + iPureIntro. repeat split. all: auto.
-                 - (* The post-condition of the IH implies the original post. *)
-                   iNext ; iIntros (v) "(%v' & v' & %h')".
-                   iExists _. iFrame.
-                   iPureIntro. intro h''. do 2 f_equal. apply h'. inversion h''. done.
-            }
-            iLöb as "IH".
-            iIntros (j i imax1 imax2 amax1 amax2 vcur1 vcur2 Φ) "(maxI1 & maxI2 & maxA1 & maxA2 & cur1 & cur2 & ε & rnm' & %maxcur1 & %maxcur2 & %imax12 & %iN) HΦ".
-            rewrite {4}/rnm_body. wp_pures.
-            rewrite {3}/rnm_body. tp_pures ; [cbv ; auto|].
-            case_bool_decide (#i = #N).
-            - tp_pures. wp_pures. tp_load ; wp_load. iApply "HΦ". iExists imax2. iFrame "rnm'". iPureIntro.
-              intros ij1. inversion H.
-              try lia.
-            - tp_pures ; wp_pures.
-              rewrite -/(rnm_body _ _ _ _ _ _ _ maxA1 _).
-              rewrite -/(rnm_body _ _ _ _ _ _ _ maxA2 _).
-              tp_bind (evalQ _ _).
-              wp_bind (evalQ _ _).
-              iAssert ({{{⌜True⌝}}} evalQ #i (inject db) {{{ v, RET v; ∃ z : Z, ⌜v = #z⌝ }}})%I as "wp_ev". 1: admit.
-              iApply "wp_ev" => // ; iIntros "!> % [%e1 ->]" ; iClear "wp_ev".
-              iAssert (∀ K, ⤇ fill K (evalQ #i (inject db')) -∗ spec_update top (∃ z : Z, ⤇ fill K #z))%I as "tp_ev". 1: admit.
-              iMod ("tp_ev" with "rnm'") as "[%e2 rnm']" => /= ; iClear "tp_ev".
-              destruct (make_decision (i = j)) as [e|n].
-              + tp_bind (Laplace _ _ _).
-                wp_bind (Laplace _ _ _).
-                (* the Laplace sampling should preserve the two assumptions that
-           if (the value stored at maxA1) < (the value stored at cur1)
-           then (the val stored at maxI1) = i
-         and
-           if (the value stored at maxA2) < (the value stored at cur2)
-           then (the val stored at maxI1) = i
-         i.e., preserve
-  maxcur1 : (amax1 < vcur1)%Z → imax1 = i
-  maxcur2 : (amax2 < vcur2)%Z → imax1 = i
-         where vcur1 and vcur2 are updated to be `a`, the result of the sampling
-                 *)
-                iApply (wp_couple_laplace e1 e2 0%Z 1%Z with "[$rnm' ε]") => //.
-                {
-                  (* sensitivity of evalQ *)
-                  admit.
-                }
-                { case_bool_decide. 2: lia.
-                  (* would be fine if we had phrased the adjacency of db and db' as dDB db db' <= 1. *)
-                  admit.
-                }
-                iNext ; iIntros (a) "rnm'" => /=.
-                wp_pures. tp_pures. rewrite !Zplus_0_r.
-                tp_store ; tp_pures ; wp_store.
-                (* both samplings resolve to the same `a`, so the implications above become... *)
-                assert (amax1 < a → imax1 = i)%Z as amax1_i.
-                {
-                  intros.
-                }
-                assert (amax2 < a → imax1 = i)%Z as amax2_i by admit.
-                tp_load ; wp_load ; tp_pures ; wp_pures.
-                case_bool_decide (amax1 < a)%Z as case_l ; tp_pures ; wp_pures.
-                all: case_bool_decide as case_r ; tp_pures ; wp_pures.
-                * do 2 (tp_store ; tp_pures ; wp_store ; wp_pures).
-                  iMod ec_zero as "ε0".
-                  iApply ("IH" $! j with "[-HΦ]") ; iFrame.
-                  rewrite e. case_bool_decide ; try lia. iFrame.
-                  iPureIntro. intuition lia.
-                * iMod ec_zero as "ε0".
-                  wp_store ; wp_pures ; wp_store ; wp_pures.
-                  iSpecialize ("IH" $! j (i+1)%Z i imax2 a amax2 a a).
-                  iSpecialize ("IH" with "[ε0 $rnm' $maxA1 $maxA2 $maxI1 $maxI2 $cur1 $cur2]").
-                  2: iApply ("IH" with "[HΦ]") ; iFrame.
-                  iSplitL. 1: case_bool_decide ; try lia ; iFrame "ε0".
-                  iPureIntro ; split ; [|split ; [|split]].
-                  1,2,4: intuition lia.
-
-                  (* to show: the outputs are equal. we updated the left but not the right. *)
-
-                  assert
-                    (forall DB (adj : DB → DB → Prop) db1 db2 i1 i2 output1 output2 max1 max2 cur1 cur2 N k,
-                        (((adj db1 db2 /\
-                           i1 = i2 /\
-                           output1 = output2 /\
-                           (max1 < cur1 ->
-                            output1 = i1) /\
-                           (max2 < cur2 ->
-                            output1 = i1) /\
-                           i1 < N /\
-                           k = N - i1 - 1 /\
-                           N - i1 - 1 <= N /\
-                           cur1 = cur2) /\
-                          max1 < cur1) /\
-                         (¬ (max2 < cur2))) ->
-                        (let max_L := cur1 in
-                         let output_L := i1 in
-                         let i_R := i2 + 1 in
-                         let i_L := i1 + 1 in
-                         (adj db1 db2 /\
-                          (i_L = i_R /\ output_L = output2) /\
-                          (max_L < cur1 -> output_L = i_L) /\
-                          (max2 < cur2 -> output_L = i_L)) /\
-                         (i_L < N <-> i_R < N) /\ N - i_L - 1 < k)
-                    )%Z.
-                  {
-                    clear.
-                    intros.
-                    destruct H as (((adj12 & i12 & out12 & outi1 & outi2 & i1N & kN & NN & cur12) & maxcur1) &  maxcur2).
-                    repeat split.
-                    1: assumption.
-                    all: try (intros ; exfalso ; by lia).
-                    1,3,4,5: try by lia.
-
-                    symmetry.
-                    (* the new left output is the current loop index i *)
-                    unfold output_L.
-                    (* the old right output is equal to the old left output *)
-                    rewrite -out12.
-                    (* that one in turn is equal to i if the current left max is below the current left sampled value *)
-                    apply outi1.
-                    (* and the left sampled value is indeed larger than the left max *)
-                    exact maxcur1.
-                  }
-
-                  symmetry.
-                  (* the old right output was equal to the old left *)
-                  rewrite -imax12.
-                  (* the old left is i if amax1 < a *)
-                  (* this doesn't make sense? the old left doesn't care about the current a *)
-                  apply amax1_i.
-                  exact case_l.
-
-                * iMod ec_zero as "ε0".
-                  tp_store ; tp_pures ; tp_store ; tp_pures.
-                  iApply ("IH" $! j with "[-HΦ]") ; [|by iFrame].
-                  (* we need 0 credits for the IH since we just dealt with the case i=j, so i+1 <> j. *)
-                  rewrite e ; case_bool_decide as Si_j ; try lia.
-                  iFrame "rnm' ε0".
-
-                  assert
-                    (forall DB (adj : DB → DB → Prop) db1 db2 i1 i2 output1 output2 max1 max2 cur1 cur2 N k,
-                        (((adj db1 db2 /\
-                           i1 = i2 /\ output1 = output2 /\
-                           (max1 < cur1 ->
-                            output1 = i1) /\
-                           (max2 < cur2 ->
-                            output1 = i1) /\
-                           i1 < N /\
-                           k = N - i1 - 1 /\
-                           N - i1 - 1 <= N /\ cur1 = cur2) /\
-                          max1 < cur1) /\
-                         ((max2 < cur2) -> False)) ->
-                        (let i_R := i2 + 1 in
-                         let i_L := i1 + 1 in
-                         (output1 = output2 /\ adj db1 db2 /\
-                          (i_L = i_R /\ i1 = output2) /\
-                          (cur1 < cur1 -> i1 = i_L) /\
-                          (max2 < cur2 -> i1 = i_L)) /\
-                         (i_L < N <-> i_R < N) /\ N - i_L - 1 < k)
-                    )%Z.
-                  {
-                    clear.
-                    intros.
-                    destruct H as (((adj12 & i12 & out12 & outi1 & outi2 & i1N & kN & NN & cur12) & maxcur1) &  maxcur2).
-                    repeat split.
-                    1: assumption.
-                    all: try (intros ; exfalso ; by lia).
-                    all: try by lia.
-                    done.
-                  }
-                  clear H0.
-                  iFrame. iPureIntro. repeat split. 1,2: intuition try lia.
-                  subst. apply amax2_i. done.
-                (*         intros Sj_N jj.
-           subst.
-   admit. *)
-
-                * iMod ec_zero as "ε0".
-                  iApply ("IH" $! j with "[-HΦ]") ; iFrame.
-                  rewrite e. case_bool_decide ; try lia. iFrame.
-                  iFrame. iPureIntro. repeat split. 1,2: intuition try lia.
-                  (* intros.
-           admit. *)
-                  done.
-
-              + tp_bind (Laplace _ _ _).
-                wp_bind (Laplace _ _ _).
-                iMod ec_zero as "ε0".
-                iApply (wp_couple_laplace e1 e2 (e2 - e1)%Z 0%Z with "[$rnm' ε0]") => //.
-                {
-                  eapply Zabs_ind ; intuition lia.
-                }
-                1: rewrite Rmult_0_l => //.
-                iNext ; iIntros (a) "rnm'" => /=.
-                wp_pures. tp_pures. tp_store ; tp_pures ; wp_store.
-                assert (amax1 < a → imax1 = i)%Z as amax1_i by admit.
-                assert (amax2 < a + (e2 - e1) → imax1 = i)%Z as amax2_i by admit.
-
-                tp_load ; wp_load ; tp_pures ; wp_pures.
-                destruct_decide (@bool_decide_reflect (amax1 < a)%Z _) as case_l.
-                all: destruct_decide (@bool_decide_reflect (amax2 < a + (e2 - e1))%Z _) as case_r.
-                all: tp_pures ; wp_pures.
-
-                * do 2 (tp_store ; tp_pures ; wp_store ; wp_pures).
-                  iApply ("IH" $! j (i+1)%Z i with "[-HΦ]") ; iFrame.
-                  repeat case_bool_decide ; try lia ; iFrame.
-                  all: iPureIntro ; intuition lia.
-                * wp_store ; wp_pures ; wp_store ; wp_pures.
-                  iApply ("IH" $! j (i+1)%Z with "[-HΦ]") ; iFrame.
-                  iSplitL. 1: repeat case_bool_decide ; try lia ; iFrame.
-                  all: iPureIntro ; intuition try lia.
-                * tp_store ; tp_pures ; tp_store ; tp_pures.
-                  iApply ("IH" $! j (i+1)%Z with "[-HΦ]") ; iFrame.
-                  iSplitL. 1: repeat case_bool_decide ; try lia ; iFrame.
-                  all: iPureIntro ; intuition lia.
-                (* 1,2: admit. *)
-                * iApply ("IH" $! j (i+1)%Z with "[-HΦ]") ; iFrame.
-                  repeat case_bool_decide ; try lia ; iFrame.
-                  all: iPureIntro ; intuition lia.
-
-          Admitted.
-
-          Lemma rnm_diffpriv_3 num den :
-            (0 < IZR num / IZR den) →
-            ∀ (K : list (ectxi_language.ectx_item prob_ectxi_lang)),
-              {{{ ⤇ fill K (report_noisy_max num den evalQ #2 (inject db')) ∗
-                  ↯ (IZR num / IZR den)
-                    (* ↯ 0 *)
-              }}}
-                (report_noisy_max num den evalQ #2 (inject db))
-                {{{ (v : val), RET v; ⤇ fill K v }}}.
-          Proof.
-            iIntros (???) "[rnm' ε] hφ".
-            rewrite /report_noisy_max.
-            simpl.
-            tp_pures.
-            tp_alloc as maxI2 "maxI2". tp_pures. tp_alloc as maxA2 "maxA2". do 5 tp_pure.
-            wp_pures. wp_alloc maxI1 as "maxI1". wp_alloc maxA1 as "maxA1". do 5 wp_pure.
-            wp_rec. wp_pures.
-            tp_pures. 1: cbv ; auto.
-            rewrite {2 4}/evalQ. tp_pures. 1: cbv ; auto. wp_pures.
-            rewrite /count_under_40/setsum/setmap/under_40/age. wp_pures. tp_pures.
-
-
-            wp_bind (Laplace _ _ _). tp_bind (Laplace _ _ _).
-            iMod ec_zero as "ε0".
-            unshelve iApply (wp_couple_laplace 1 2 1 0 _ (num) (2*den) _ _  (AppRCtx _ :: K)
-                with "[ε0 $rnm']" ) => //=.
-            1: by cbv.
-            { rewrite mult_IZR.
-              rewrite Rmult_comm.
-              rewrite Rdiv_mult_distr.
-              rewrite {1}/Rdiv.
-              revert H.
-              set (r := (IZR num / IZR den)).
-              lra.
-            }
-            1: rewrite Rmult_0_l => //.
-            simpl. tp_pures.
-            iIntros "!> %z f'" => /=. wp_pures. tp_pures. tp_load ; wp_load. wp_pures.
-            wp_load. tp_pures. tp_load. tp_pures. 1: cbv ; auto. wp_pures.
-            tp_store. tp_pures. tp_store. do 2 wp_store. wp_pures. tp_pures. 1: cbv ; auto.
-            rewrite {2 4}/evalQ. tp_pures. 1,2: cbv ; auto. wp_pures.
-            rewrite /count_over_80/setsum/setmap/over_80/age. wp_pures. tp_pures.
-            wp_bind (Laplace _ _ _). tp_bind (Laplace _ _ _).
-            iMod ec_zero as "ε0".
-            unshelve iApply (wp_couple_laplace _ _ 0 0 _ (num) (2*den) _ _  (AppRCtx _ :: K)
-                with "[ε ε0 $f']" ) => //=.
-            1: by cbv.
-            { rewrite mult_IZR.
-              rewrite Rmult_comm.
-              rewrite Rdiv_mult_distr.
-              rewrite {1}/Rdiv.
-              revert H.
-              set (r := (IZR num / IZR den)).
-              lra.
-            }
-            (* 1: rewrite Rmult_1_l => //. 1:admit. *)
-            1: rewrite Rmult_0_l => //.
-            simpl. tp_pures.
-            iIntros "!> %z2 f'" => /=. wp_pures. tp_pures. tp_load ; wp_load. wp_pures.
-            wp_load. wp_pures.
-            tp_pures. tp_load. tp_pures ; [cbv ; auto|].
-            rewrite !Zplus_0_r ?Zplus_0_l.
-            case_bool_decide.
-            - do 2 wp_store. wp_pures.
-              tp_pures. tp_store ; tp_pures ; tp_store ; tp_pures.
-              1: cbv ; auto. tp_load.
-              wp_load.
-              iApply "hφ". done.
-              Unshelve.
-              2: f_equal. simpl.
-            - wp_pures.
-              tp_pures.
-              1: cbv ; auto. tp_load.
-              wp_load.
-              iApply "hφ". done.
-              Unshelve.
-              all: f_equal.
-          Qed.
+       wp_bind (Laplace _ _ _). tp_bind (Laplace _ _ _).
+       iMod ec_zero as "ε0".
+       unshelve iApply (wp_couple_laplace 1 2 1 0 _ (num) (2*den) _ _  (AppRCtx _ :: K)
+           with "[ε0 $rnm']" ) => //=.
+       1: by cbv.
+       { rewrite mult_IZR.
+         rewrite Rmult_comm.
+         rewrite Rdiv_mult_distr.
+         rewrite {1}/Rdiv.
+         revert H.
+         set (r := (IZR num / IZR den)).
+         lra.
+       }
+       1: rewrite Rmult_0_l => //.
+       simpl. tp_pures.
+       iIntros "!> %z f'" => /=. wp_pures. tp_pures. tp_load ; wp_load. wp_pures.
+       wp_load. tp_pures. tp_load. tp_pures. 1: cbv ; auto. wp_pures.
+       tp_store. tp_pures. tp_store. do 2 wp_store. wp_pures. tp_pures. 1: cbv ; auto.
+       rewrite {2 4}/evalQ. tp_pures. 1,2: cbv ; auto. wp_pures.
+       rewrite /count_over_80/setsum/setmap/over_80/age. wp_pures. tp_pures.
+       wp_bind (Laplace _ _ _). tp_bind (Laplace _ _ _).
+       iMod ec_zero as "ε0".
+       unshelve iApply (wp_couple_laplace _ _ 0 0 _ (num) (2*den) _ _  (AppRCtx _ :: K)
+           with "[ε ε0 $f']" ) => //=.
+       1: by cbv.
+       { rewrite mult_IZR.
+         rewrite Rmult_comm.
+         rewrite Rdiv_mult_distr.
+         rewrite {1}/Rdiv.
+         revert H.
+         set (r := (IZR num / IZR den)).
+         lra.
+       }
+       (* 1: rewrite Rmult_1_l => //. 1:admit. *)
+       1: rewrite Rmult_0_l => //.
+       simpl. tp_pures.
+       iIntros "!> %z2 f'" => /=. wp_pures. tp_pures. tp_load ; wp_load. wp_pures.
+       wp_load. wp_pures.
+       tp_pures. tp_load. tp_pures ; [cbv ; auto|].
+       rewrite !Zplus_0_r ?Zplus_0_l.
+       case_bool_decide.
+       - do 2 wp_store. wp_pures.
+         tp_pures. tp_store ; tp_pures ; tp_store ; tp_pures.
+         1: cbv ; auto. tp_load.
+         wp_load.
+         iApply "hφ". done.
+         Unshelve.
+         2: f_equal. simpl.
+       - wp_pures.
+         tp_pures.
+         1: cbv ; auto. tp_load.
+         wp_load.
+         iApply "hφ". done.
+         Unshelve.
+         all: f_equal.
+     Qed. *)
 
 End rnm.
